concurrency/scheduler.v
@@ -13,13 +13,17 @@ End NatTID.
 Module Type Scheduler (TID:ThreadID).
   Import TID.
   Parameter schedule : Type.
+  Parameter empty : schedule.
   Parameter schedPeek: schedule -> option tid.
   Parameter schedSkip: schedule -> schedule.
+  Parameter buildSched: list tid -> schedule.
 End Scheduler.
 
 Module ListScheduler (TID:ThreadID) <: Scheduler TID .
   Import TID.
   Definition schedule:= list tid.
+  Definition empty : schedule := nil.
   Definition schedPeek (sc:schedule):= @List.hd_error tid sc.
   Definition schedSkip (sc:schedule): schedule:= @List.tl tid sc.
+  Definition buildSched (ls : list tid) : schedule := ls.
 End ListScheduler.
