Makefile
@@ -127,7 +127,7 @@ SEPCOMP_FILES= \
 CONCUR_FILES= \
   sepcomp.v threads_lemmas.v permissions.v\
   pos.v scheduler.v \
-  concurrent_machine.v juicy_machine.v \
+  concurrent_machine.v juicy_machine.v dry_machine.v \
   compcert_threads.v compcert_threads_lemmas.v \
   erasure.v 
 
